Risc0/Gadgets/IsZero/Constraints/WeakestPresPart0.lean
@@ -9,21 +9,14 @@ open MLIRNotation
 
 -- The state obtained by running Code.part0 on st
 def part0_state (st: State) : State :=
-  
-        ((((st[props][{ name := "%1" : PropVar }] ← True)["%2"] ←ₛ
-              getImpl st { name := "in" : BufferVar } (0 : Back) (0 : ℕ))[props][{ name := "%4" : PropVar }] ←
-            (Option.get!
-                (State.props
-                  ((st[props][{ name := "%1" : PropVar }] ← True)["%2"] ←ₛ
-                    getImpl st { name := "in" : BufferVar } (0 : Back) (0 : ℕ))
-                  { name := "%1" : PropVar }) ∧
-              Option.get!
-                  (State.felts
-                    ((st[props][{ name := "%1" : PropVar }] ← True)["%2"] ←ₛ
-                      getImpl st { name := "in" : BufferVar } (0 : Back) (0 : ℕ))
-                    { name := "%2" : FeltVar }) =
-                (0 : Felt)))["%3"] ←ₛ
-          getImpl st { name := "data" : BufferVar } (0 : Back) (0 : ℕ)) 
+  if Γ st ⟦Code.part0⟧.isFailed = true
+  then {st with isFailed := true}
+  else ((((st[props][{ name := "%1" : PropVar }] ← True)[felts][{ name := "%2" : FeltVar }] ←
+          Option.get!
+            (Buffer.back st { name := "in" : BufferVar } (0 : Back) (0 : ℕ)))[props][{ name := "%4" : PropVar }] ←
+        Option.get! (Buffer.back st { name := "in" : BufferVar } (0 : Back) (0 : ℕ)) =
+          (0 : Felt))[felts][{ name := "%3" : FeltVar }] ←
+      Option.get! (Buffer.back st { name := "data" : BufferVar } (0 : Back) (0 : ℕ)))
 
 def part0_drops (st: State) : State :=
   st
@@ -37,12 +30,81 @@ lemma part0_wp {st : State} :
   Code.getReturn (Γ st ⟦Code.part0;Code.part1;dropfelt ⟨"%3"⟩;Code.part2;dropfelt ⟨"%2"⟩;dropfelt ⟨"%0"⟩;dropfelt ⟨"%6"⟩;dropfelt ⟨"%7"⟩;dropfelt ⟨"%8"⟩;dropfelt ⟨"%9"⟩⟧)↔
   Code.getReturn (part0_state_update st) := by
   generalize eq : (Code.part1;dropfelt ⟨"%3"⟩;Code.part2;dropfelt ⟨"%2"⟩;dropfelt ⟨"%0"⟩;dropfelt ⟨"%6"⟩;dropfelt ⟨"%7"⟩;dropfelt ⟨"%8"⟩;dropfelt ⟨"%9"⟩) = prog
-  unfold Code.part0
-  MLIR
-  rewrite [←eq]
-  
-  unfold part0_state_update part0_drops part0_state
-  rfl
+  rewrite [MLIR.run_seq_def]
+  unfold part0_state_update
+  rewrite [eq]
+  by_cases hIsFailed: (Γ st ⟦Code.part0⟧).isFailed
+  . have hFailedFull : (Γ (Γ st ⟦Code.part0⟧) ⟦prog⟧).isFailed = true := by simp [MLIR.isFailed_monotonic, hIsFailed]
+    unfold Code.getReturn
+    simp [hFailedFull]
+    intro
+    unfold part0_state part0_drops
+    simp [hIsFailed, MLIR.isFailed_monotonic]
+  . have h_SameIfValid : (Γ st ⟦Code.part0⟧) = (part0_drops (part0_state st)) := by
+      have h_SAVE: ¬Γ st ⟦Code.part0⟧.isFailed = true := hIsFailed --REVIEW another way to duplicate a goal?
+      generalize eq_st': Γ st ⟦Code.part0⟧ = st'
+      rewrite [eq_st'] at hIsFailed
+      unfold Code.part0 at eq_st'
+      -- MLIR START --REVIEW how to target our tactics at a hypothesis
+      rewrite [MLIR.run_seq_def] at eq_st'
+      repeat (
+        first
+        | rewrite [MLIR.run_ass_def] at eq_st'
+        | rewrite [MLIR.run_set_def] at eq_st'
+        | rewrite [MLIR.run_if] at eq_st'
+        | rewrite [MLIR.run_nondet] at eq_st'
+        | rewrite [MLIR.run_eqz] at eq_st'
+        | rewrite [MLIR.run_dropfelt] at eq_st'
+      )
+      -- simp only [
+      --   Op.eval_const, Op.eval_true, Op.eval_getBuffer, Op.eval_add, Op.eval_sub,
+      --   Op.eval_mul, Op.eval_isz, Op.eval_inv, Op.eval_andEqz, Op.eval_andCond
+      -- ] at eq_st'
+      rewrite [MLIR.run_seq_def] at eq_st'
+      repeat (
+        first
+        | rewrite [MLIR.run_ass_def] at eq_st'
+        | rewrite [MLIR.run_set_def] at eq_st'
+        | rewrite [MLIR.run_if] at eq_st'
+        | rewrite [MLIR.run_nondet] at eq_st'
+        | rewrite [MLIR.run_eqz] at eq_st'
+        | rewrite [MLIR.run_dropfelt] at eq_st'
+      )
+      -- simp only [
+      --   Op.eval_const, Op.eval_true, Op.eval_getBuffer, Op.eval_add, Op.eval_sub,
+      --   Op.eval_mul, Op.eval_isz, Op.eval_inv, Op.eval_andEqz, Op.eval_andCond
+      -- ] at eq_st'
+      rewrite [MLIR.run_seq_def] at eq_st'
+      repeat (
+        first
+        | rewrite [MLIR.run_ass_def] at eq_st'
+        | rewrite [MLIR.run_set_def] at eq_st'
+        | rewrite [MLIR.run_if] at eq_st'
+        | rewrite [MLIR.run_nondet] at eq_st'
+        | rewrite [MLIR.run_eqz] at eq_st'
+        | rewrite [MLIR.run_dropfelt] at eq_st'
+      )
+      simp only [
+        Op.eval_const, Op.eval_true, Op.eval_getBuffer, Op.eval_add, Op.eval_sub,
+        Op.eval_mul, Op.eval_isz, Op.eval_inv, Op.eval_andEqz, Op.eval_andCond
+      ] at eq_st'
+      try simp only [Buffer.back_def.symm, isGetValid_def.symm, getImpl_def.symm, State.update_val', State.update_constr'] at eq_st'
+      try simp [getImpl_skip_set_offset] at eq_st'
+      --MLIR END
+
+      --SIMPLIFY VALID START (2 gets means 2 rewrites using simplify_valid_get)
+      rewrite [←eq_st'] at hIsFailed
+      try simp only [State.updateFelts_isFailed, State.updateProps_isFailed] at hIsFailed
+      rewrite [simplify_valid_get hIsFailed] at eq_st' hIsFailed
+      try simp only [State.updateFelts_isFailed, State.updateProps_isFailed] at hIsFailed
+      rewrite [simplify_valid_get hIsFailed] at eq_st' hIsFailed
+      --SIMPLIFY VALID END
+      rewrite [←eq_st']
+      MLIR
+      unfold part0_drops part0_state
+      simp only [h_SAVE, ite_false]
+
+    rw [h_SameIfValid]
 
 lemma part0_cumulative_wp {x0 y0 y1: Felt}:
   Code.run (start_state [x0] ([y0,y1])) ↔
