Risc0/Gadgets/IsZero/Constraints/WeakestPresPart2.lean
@@ -135,6 +135,6 @@ lemma closed_form {x0 y0 y1: Felt} :
     -- there are statements after an if
     try simp [State.buffers_if_eq_if_buffers,State.bufferWidths_if_eq_if_bufferWidths,State.constraints_if_eq_if_constraints,State.cycle_if_eq_if_cycle,State.felts_if_eq_if_felts,State.isFailed_if_eq_if_isFailed,State.props_if_eq_if_props,State.vars_if_eq_if_vars]
     unfold Code.getReturn
-    simp only
+    simp only [State.updateProps_isFailed, and_true]
     simp only [Code.getReturn, State.constraintsInVar, State.updateProps_props_get_wobbly, Option.getD_some]
 end Risc0.IsZero.Constraints.WP
